Add indexed monad instances and `Cava` class dependency on `cava`

cava/Cava/Core/StateMonadAST.v
@@ -15,75 +15,94 @@
 (****************************************************************************)
 
 Require Import Coq.Lists.List.
-Require Import ExtLib.Structures.Monads.
-Import ListNotations.
-Require Import Cava.Core.Signal.
 
+Require Import ExtLib.Structures.Monoid.
+Require Import ExtLib.Data.List.
+Import ListNotations.
+
+Require Import Cava.Core.Signal.
 Require Import Cava.Util.Vector.
 Require Import Cava.Util.Tactics.
+Require Import Cava.Util.IxMonad.
+
+Import IxMonadNotation.
+Open Scope ix_monad_scope.
 
 Section WithSignal.
   Context {signal : SignalType -> Type}.
 
-  Inductive cava : list SignalType -> Type -> Type :=
-  | Ret : forall {t} (x : t), cava [] t
+  (* TODO(blaxill):
+     - If we move to delayless loop, this will be the deep embedding of monad fix + delay.
+     - Delay could possibly be merged into Ret, if Ret is generalized to add state
+   *)
+
+  Inductive CavaSpine : list SignalType -> Type -> Type :=
+  | Ret : forall {t} (x : t), CavaSpine [] t
   | LoopInit :
       forall {i s o body_state}
         (resetval : combType s)
-        (body : i * signal s -> cava body_state (o * signal s))
+        (body : i * signal s -> CavaSpine body_state (o * signal s))
         (input : i),
-        cava (s :: body_state) o
-  | DelayInit : forall {s} (resetval : combType s) (x : signal s), cava [s] (signal s)
+        CavaSpine (s :: body_state) o
+  | DelayInit : forall {s} (resetval : combType s) (x : signal s), CavaSpine [s] (signal s)
   | Bind :
-      forall {t u xs fs} (x : cava xs t) (f : t -> cava fs u),
-        cava (xs ++ fs) u
+      forall {t u xs fs} (x : CavaSpine xs t) (f : t -> CavaSpine fs u),
+        CavaSpine (xs ++ fs) u
   .
-  Notation "x <- c1 ;; c2" := (Bind c1 (fun x => c2)) (at level 61, c1 at next level, right associativity).
 
-  (* derived loop/delay with default initial state *)
-  Definition Loop {i s o body_state} body input :=
-    @LoopInit i s o body_state (defaultCombValue _) body input.
-  Definition Delay {s} (x : signal s) := DelayInit (defaultCombValue _) x.
-
-  (* composition *)
-  Definition compose {i t o s1 s2} (f : i -> cava s1 t) (g : t -> cava s2 o) (input : i)
-    : cava (s1 ++ s2) o :=
-    x <- f input ;;
-    g x.
-  Infix ">=>" := compose (at level 40).
-
-  Definition fork2 {t} (x : t) : cava [] (t * t) := Ret (x,x).
+  Instance cava_IxMonad : IxMonad Monoid_list_app CavaSpine :=
+  { ret _ x := Ret x;
+    bind _ _ _ _ x f := Bind x f;
+  }.
 
   Class Cava :=
-    { xor2  : signal Bit * signal Bit -> cava [] (signal Bit);
-      inv : signal Bit -> cava [] (signal Bit) }.
+    { cava : list SignalType -> Type -> Type;
+      monad :> IxMonad Monoid_list_app cava;
+      xor2  : signal Bit * signal Bit -> cava [] (signal Bit);
+      inv : signal Bit -> cava [] (signal Bit);
+      loop_init : forall {i s o body_state}
+        (resetval : combType s)
+        (body : i * signal s -> cava body_state (o * signal s))
+        (input : i),
+        cava (s :: body_state) o;
+      delay_init : forall {s}
+        (resetval : combType s)
+        (x : signal s),
+        cava [s] (signal s);
+   }.
 
   Context {semantics:Cava}.
 
+  Definition delay {s} (x : signal s) := delay_init (defaultCombValue _) x.
+  Definition loop {i s o body_state} body input :=
+    @loop_init _ i s o body_state (defaultCombValue _) body input.
+  Definition fork2 {t} (x : t) : cava [] (t * t) := ret (x,x).
+
   (* test circuits *)
-  Definition test : signal Bit -> cava [Bit] (signal Bit) := Loop (xor2 >=> fork2).
+  Definition test : signal Bit -> cava [Bit] (signal Bit) := loop (xor2 >=> fork2).
+  (* Set Printing Notations. *)
   Definition test2 (i : signal Bit) : cava [Bit;Bit] (signal Bit) :=
-    Loop
-      (Loop
+    loop
+      (loop
          (fun '(i,r1,r2) =>
             r1' <- xor2 (i, r1) ;;
-            r2' <- xor2 (r1', r2) ;;
-            Ret (r2',r1',r2'))) i.
+            r2' <- xor2 (r1, r2) ;;
+            ret (r2',r1',r2))) i.
 
   (* same as test2, but with initial values undetermined *)
   Definition test2_init (r1_init r2_init : combType Bit)
              (i : signal Bit) : cava [Bit;Bit] (signal Bit) :=
-    LoopInit r1_init
-             (LoopInit r2_init
+    loop_init r1_init
+             (loop_init r2_init
                        (fun '(i,r1,r2) =>
                           r1' <- xor2 (i, r1) ;;
                           r2' <- xor2 (r1', r2) ;;
-                          Ret (r2',r1',r2'))) i.
+                          ret (r2',r1',r2'))) i.
 
   (* test expressions; make sure notation works as intended *)
   Check (test >=> test >=> inv). (* compose sequential and combinational circuits *)
   Check (fun i =>
-           x <- Loop (xor2 >=> fork2) i ;;
+           x <- loop (xor2 >=> fork2) i ;;
            inv x). (* loop bind *)
 
 
@@ -114,86 +133,94 @@ Section WithSignal.
 
 End WithSignal.
 
-(* from now assume cava is combinational (later this would be done with Cava instance) *)
-Let cava := @cava combType.
+Section Eval.
+  (* from now assume cava is combinational (later this would be done with Cava instance) *)
+  Let CavaSpine := @CavaSpine combType.
 
-(* mealy machine interpretation (single-step)
+  (* mealy machine interpretation (single-step)
 
-     if reset=true, then the state values are ignored and output is computed
-     based on register reset values *)
-Fixpoint step {o ts} (reset : bool) (c : cava ts o)
-  : signal_values ts -> o * signal_values ts :=
-  match c with
-  | Ret x => fun _ => (x,tt)
-  | Bind x f =>
-    fun s =>
-      let '(s1,s2) := split_values s in
-      let '(y,s1') := step reset x s1 in
-      let '(z,s2') := step reset (f y) s2 in
-      (z, combine_values s1' s2')
-  | LoopInit resetval body input =>
-    fun s =>
-      let s1 := if reset then resetval else fst s in
-      let '(out,s1',s2') := step reset (body (input, s1)) (snd s) in
-      (out, (s1', s2'))
-  | DelayInit resetval x =>
-    fun s =>
-      let s1 := if reset then resetval else fst s in
-      (s1, (x,tt))
-  end.
+       if reset=true, then the state values are ignored and output is computed
+       based on register reset values *)
+  Fixpoint step {o ts} (reset : bool) (c : CavaSpine ts o)
+    : signal_values ts -> o * signal_values ts :=
+    match c with
+    | Ret x => fun _ => (x,tt)
+    | Bind x f =>
+      fun s =>
+        let '(s1,s2) := split_values s in
+        let '(y,s1') := step reset x s1 in
+        let '(z,s2') := step reset (f y) s2 in
+        (z, combine_values s1' s2')
+    | LoopInit resetval body input =>
+      fun s =>
+        let s1 := if reset then resetval else fst s in
+        let '(out,s1',s2') := step reset (body (input, s1)) (snd s) in
+        (out, (s1', s2'))
+    | DelayInit resetval x =>
+      fun s =>
+        let s1 := if reset then resetval else fst s in
+        (s1, (x,tt))
+    end.
 
-Fixpoint default_values {ts} : signal_values ts :=
-  match ts with
-  | [] => tt
-  | t :: ts => (defaultCombValue t, default_values)
-  end.
+  Fixpoint default_values {ts} : signal_values ts :=
+    match ts with
+    | [] => tt
+    | t :: ts => (defaultCombValue t, default_values)
+    end.
 
-(* circuit simulation with initial state *)
-Definition simulate_init {i ts o} (c : i -> cava ts o) (input : list i)
-           (init : signal_values ts) : list o :=
-  fst (fold_left (fun '(acc,s) i =>
-                    let '(o,s') := step false (c i) s in
-                    (acc ++ [o], s'))
-                 input ([], init)).
+  (* circuit simulation with initial state *)
+  Definition simulate_init {i ts o} (c : i -> CavaSpine ts o) (input : list i)
+             (init : signal_values ts) : list o :=
+    fst (fold_left (fun '(acc,s) i =>
+                      let '(o,s') := step false (c i) s in
+                      (acc ++ [o], s'))
+                   input ([], init)).
 
-(* circuit simulation *)
-Definition simulate {i ts o} (c : i -> cava ts o) (input : list i) : list o :=
-  match input with
-  | [] => []
-  | i0 :: input =>
-    (* initial step is called with reset=true *)
-    let '(o,state) := step true (c i0) default_values in
-    o :: simulate_init c input state
-  end.
+  (* circuit simulation *)
+  Definition simulate {i ts o} (c : i -> CavaSpine ts o) (input : list i) : list o :=
+    match input with
+    | [] => []
+    | i0 :: input =>
+      (* initial step is called with reset=true *)
+      let '(o,state) := step true (c i0) default_values in
+      o :: simulate_init c input state
+    end.
 
-Instance CombinationalSemantics : @Cava combType :=
-  {| xor2 := fun i => Ret (xorb (fst i) (snd i));
-     inv := fun i => Ret (negb i) |}.
+  Existing Instance cava_IxMonad.
+  Instance CombinationalSemantics : @Cava combType :=
+    {| cava := CavaSpine;
+       xor2 := fun i => Ret (xorb (fst i) (snd i));
+       inv := fun i => Ret (negb i) ;
+       loop_init := @LoopInit _;
+       delay_init := @DelayInit _;
+    |}.
 
-(* t   0 1 2 3 4 5 6
-     in  1 1 1 1 1 1 1
-     reg 0 1 0 1 0 1 0
-     out 1 0 1 0 1 0 1 *)
-Compute (simulate test (repeat true 10)).
-(*      = [true; false; true; false; true; false; true; false; true; false] *)
+  (* t   0 1 2 3 4 5 6
+       in  1 1 1 1 1 1 1
+       reg 0 1 0 1 0 1 0
+       out 1 0 1 0 1 0 1 *)
+  Compute (simulate test (repeat true 10)).
+  (*      = [true; false; true; false; true; false; true; false; true; false] *)
 
-(* starting with r1=0, r2=0:
+  (* starting with r1=0, r2=0:
 
-     t   0 1 2 3 4 5 6
-     in  1 1 1 1 1 1 1
-     r1  0 1 0 1 0 1 0
-     r2  0 1 1 0 0 1 1
-     out 1 1 0 0 1 1 0
- *)
-Compute (simulate test2 (repeat true 10)).
-(*      = [true; true; false; false; true; true; false; false; true; true] *)
+       t   0 1 2 3 4 5 6
+       in  1 1 1 1 1 1 1
+       r1  0 1 0 1 0 1 0
+       r2  0 1 1 0 0 1 1
+       out 1 1 0 0 1 1 0
+   *)
+  Compute (simulate test2 (repeat true 10)).
+  (*      = [true; true; false; false; true; true; false; false; true; true] *)
 
-(* starting with r1=1, r2=1:
-     t   0 1 2 3 4 5 6
-     in  1 1 1 1 1 1 1
-     r1  1 0 1 0 1 0 1
-     r2  1 1 0 0 1 1 0
-     out 1 0 0 1 1 0 0
- *)
-Compute (simulate (test2_init true true) (repeat true 10)).
-(*      = [true; false; false; true; true; false; false; true; true; false] *)
+  (* starting with r1=1, r2=1:
+       t   0 1 2 3 4 5 6
+       in  1 1 1 1 1 1 1
+       r1  1 0 1 0 1 0 1
+       r2  1 1 0 0 1 1 0
+       out 1 0 0 1 1 0 0
+   *)
+  Compute (simulate (test2_init true true) (repeat true 10)).
+  (*      = [true; false; false; true; true; false; false; true; true; false] *)
+
+End Eval.
