cava/Cava/Util/IxMonad.v
@@ -1,0 +1,37 @@
+Require Import ExtLib.Structures.Monoid.
+
+(* Set Universe Polymorphism. *)
+
+(* Dominic Orchard style indexed monad *)
+(* TODO(blaxill): switch to Atkey or McBride ? *)
+Class IxMonad {x} (eff: Monoid x) (m : x -> Type -> Type) : Type :=
+{ ret : forall {a}, a -> m (monoid_unit eff) a
+; bind : forall {a b s t}, m s a -> (a -> m t b) -> m (monoid_plus eff s t) b
+}.
+
+Class IxMonadFix {x} (eff: Monoid x) (m : x -> Type -> Type) : Type :=
+{ mfix : forall {a b s}, ((a -> m s b) -> a -> m s b) -> a -> m s b }.
+
+Definition mcompose {x} {eff: Monoid x} {m} {M: IxMonad eff m}
+           {T U V:Type} {a b}
+           (f: T -> m a U) (g: U -> m b V): (T -> m (monoid_plus eff a b) V) :=
+  fun x => bind (f x) g.
+
+Module IxMonadNotation.
+  Declare Scope ix_monad_scope.
+  Delimit Scope ix_monad_scope with ix_monad.
+
+  Notation "c >>= f" := (bind c f) (at level 58, left associativity) : ix_monad_scope.
+  Notation "f =<< c" := (bind c f) (at level 61, right associativity) : ix_monad_scope.
+  Notation "f >=> g" := (mcompose f g) (at level 61, right associativity) : ix_monad_scope.
+
+  Notation "e1 ;; e2" := (bind e1%ix_monad (fun _ => e2%ix_monad))%ix_monad
+    (at level 61, right associativity) : ix_monad_scope.
+
+  Notation "x <- c1 ;; c2" := (bind c1 (fun x => c2))
+    (at level 61, c1 at next level, right associativity) : ix_monad_scope.
+
+  Notation "' pat <- c1 ;; c2" :=
+    (bind c1 (fun x => match x with pat => c2 end))
+    (at level 61, pat pattern, c1 at next level, right associativity) : ix_monad_scope.
+End IxMonadNotation.
